LL1/Proofs/ParseTableGen/EndToEnd.v
@@ -2,34 +2,35 @@ Require Import LL1.ParseTableGen.
 Require Import LL1.ParseTable.
 
 Require Import LL1.Proofs.ParseTableGen.mkNullableSet_Correctness.
+Require Import LL1.Proofs.ParseTableGen.mkFirstMap_Correctness.
 Require Import LL1.Proofs.ParseTableGen.mkEntries_Correctness.
 Require Import LL1.Proofs.ParseTableGen.mkParseTable_Correctness.
 
 Theorem genTableForGrammar_sound : 
-  forall g fi fo tbl,
-  first_map_for fi g
-  -> follow_map_for fo g
-  -> genTableForGrammar g fi fo = Some tbl
+  forall g fo tbl,
+  follow_map_for fo g
+  -> genTableForGrammar g fo = Some tbl
   -> parse_table_for tbl g.
 Proof.
-  intros g fi fo tbl Hfi Hfo Hmk.
+  intros g fo tbl Hfo Hmk.
   eapply mkParseTable_sound; eauto.
+  pose proof (mkNullableSet_correct g).
   eapply mkEntries_correct; eauto.
-  apply mkNullableSet_correct.
+  apply mkFirstMap_correct; auto.
 Qed.
 
 Theorem genTableForGrammar_complete :
-  forall g fi fo tbl,
-    first_map_for fi g
-    -> follow_map_for fo g
+  forall g fo tbl,
+    follow_map_for fo g
     -> parse_table_for tbl g
     -> exists tbl',
         ParseTable.Equal tbl tbl'
-        /\ genTableForGrammar g fi fo = Some tbl'.
+        /\ genTableForGrammar g fo = Some tbl'.
 Proof.
-  intros g fi fo tbl Hfi Hfo Hpt.
+  intros g fo tbl Hfo Hpt.
   eapply mkParseTable_complete; eauto.
+  pose proof (mkNullableSet_correct g).
   eapply mkEntries_correct; eauto.
-  apply mkNullableSet_correct.
+  apply mkFirstMap_correct; auto.
 Qed.
 
